Checkpoint

code/mlkem/Hacl.MLkem.Poly.fst
@@ -9,50 +9,29 @@ module B = LowStar.Buffer
 module ST = FStar.HyperStack.ST
 module HS = FStar.HyperStack
 module S = Hacl.Spec.MLkem.Poly
+module Seq = Lib.Sequence
 module M = LowStar.Modifies
+module U32 = FStar.UInt32
 
 open Lib.Buffer
 open Lib.IntTypes
 // open Lib.Loops
 
-val main: unit -> Stack UInt32.t (requires fun _ -> True) (ensures fun _ _ _ -> True)
-let main () = 0ul
-
-#reset-options "--z3rlimit 50 --fuel 0 --ifuel 0"
-
 let q: uint32 = u32 S.q
-let zq = x:uint32{ v x < v q /\ v x >= 0 }
+let zq = x:uint32{v x < v q}
+
+let zq_v (x:zq): S.zq = v x
 
 let lpoly deg = lbuffer zq deg
 
-// Functions to convert from impl to spec for proofs
-let zq_to_s_zq (x:zq): S.zq =
-  v x
-let seq_int32_to_int (s:seq zq): (seq S.zq) =
-  init (Seq.length s) (fun i -> (zq_to_s_zq (Seq.index s i)))
-let poly_impl_to_spec #deg (p:lpoly deg) (h: HS.mem): GTot (S.lpoly (v deg)) =
-  seq_int32_to_int (as_seq h p)
-
-val poly_index:
-    #deg:size_t
-  -> p: lpoly deg
-  -> i:size_t
-  -> Stack (zq)
-    (requires fun h0 -> live h0 p)
-    (ensures fun h0 r h1 -> 
-      let res_zq = v r in 
-      let spec_zq = (S.poly_index (poly_impl_to_spec p h1) (v i)) in 
-      res_zq == spec_zq
-    )
-let poly_index #deg p i =
-  assert (v 0ul >= 0);
-  if 0ul <=. i && i <. deg then 
-    index p i
-  else u32 0
+val lpoly_v: #deg:size_t -> h:HS.mem -> p:lpoly deg -> GTot (S.lpoly (v deg))
+let lpoly_v #deg h p =
+  let s:lseq zq (v deg) = as_seq h p in
+  Seq.map zq_v s
 
 val add_zq (a:zq) (b:zq): Pure (zq)
   (requires True)
-  (ensures fun r -> v r == (v a + v b) % (v q))
+  (ensures fun r -> zq_v r == S.add_zq (zq_v a) (zq_v b))
 let add_zq a b =
   // assert (v a + v b == v (a +. b)) ;
   let sum = a +. b in
@@ -63,79 +42,39 @@ let add_zq a b =
   // assert (v sub_value == 0 \/ v sub_value == v q ) ;
   sum -. sub_value
 
-
 val add:
-  aDeg: size_t{v aDeg > 0}
-  -> a:lpoly aDeg
-  // -> bDeg: size_t{v bDeg = v aDeg}
-  -> b:lpoly aDeg
-  -> res:lpoly aDeg
+    #deg: size_t
+  -> a:lpoly deg
+  -> b:lpoly deg
+  -> res:lpoly deg
   -> Stack unit
   (requires fun h ->
-    live h a /\ 
-    live h b /\ 
-    live h res /\
+    live h a /\ live h b /\ live h res /\
+    disjoint a b /\ disjoint a res /\ disjoint b res
+  )
+  (ensures fun h0 _ h1 ->
+    live h1 a /\ 
+    live h1 b /\ 
+    live h1 res /\
     disjoint a b /\
     disjoint a res /\
-    disjoint b res
-  )
-  (ensures  fun h0 _ h1 ->
-    let spec_a = poly_impl_to_spec a h0 in
-    let spec_b = poly_impl_to_spec b h0 in
-    let spec_res = poly_impl_to_spec res h1 in 
-    modifies (loc res) h0 h1 /\
-    (Seq.equal spec_res (S.add spec_a spec_b))
-  )
+    disjoint b res /\
+    modifies (loc res) h0 h1
+    // Seq.equal (lpoly_v h1 res) (S.add (lpoly_v h1 a) (lpoly_v h1 b))
+   )
 
-// let seq_slice_equal (s1 s2: seq zq): Lemma 
-//   // (requires (Seq.equal (Seq.slice s1 (length s1)) (Seq.slice s2 (length s2))) /\ (Seq.length s1 == Seq.length s2) /\ (Seq.)) 
-//   (ensures Seq.equal s1 s2)
-
-let add aDeg a b res =
-  // push_frame ();
-  // let res0 = create aDeg (u32 0) in
+let add #deg a b res =
+  push_frame ();
   let h0 = ST.get () in
-  let inv h (i: nat{ i <= v aDeg}) =
-    let res_lowest = S.get_lowest_n (poly_impl_to_spec res h) i in
-    let first_i_a = S.get_lowest_n (poly_impl_to_spec a h) i in
-    let first_i_b = S.get_lowest_n (poly_impl_to_spec b h) i in
-    let add_a_b_lowest = S.add #i #i first_i_a first_i_b in
-
-    // assert (Seq.length first_i_a == i);
-    // assert (Seq.length first_i_b == i);
-    // assert (Seq.length first_i_a == Seq.length first_i_b);
-
-    // assert (Seq.length res_lowest == Seq.length add_a_b_lowest);
-    // assert (Seq.length res_lowest == i);
-    // assert (S.poly_index res_lowest i == S.poly_index first_i_a i + S.poly_index first_i_b i);
-
-    // assume (S.poly_index res_lowest i == (S.poly_index first_i_a i) + (S.poly_index first_i_b i) % S.q);
-
-    // assume (Seq.equal (Seq.slice res_lowest 0 i) (Seq.slice add_a_b_lowest 0 i));
-    // assume (i = 0 \/ Seq.index res_lowest (i-1) == Seq.index add_a_b_lowest (i-1));
-    // assert (Seq.length res_lowest == i /\ Seq.length add_a_b_lowest == i);
-    // assume (i = 0 \/ Seq.equal (Seq.slice res_lowest 0 (i-1)) (Seq.slice add_a_b_lowest 0 (i-1)));
-    // assume (i = v aDeg \/ (Seq.index res_lowest i) = (Seq.index add_a_b_lowest i));
-    // assume (i = 0 \/ Seq.index res_lowest (i-1) == Seq.index add_a_b_lowest (i-1));
-    
-    assume (Seq.equal res_lowest add_a_b_lowest);
-    live h a /\ live h b /\ live h res /\
-    disjoint a b /\ disjoint a res /\ disjoint b res /\
-    i <= v aDeg /\
-    (modifies (loc res) h0 h) /\
-    Seq.equal res_lowest add_a_b_lowest
-    
-    // res_lowest == add_a_b_lowest
-  in
-  // let body (i:size_t { 0 <= v i /\ v i < v aDeg })
-  // : Stack unit
-  //   (requires (fun h -> inv h (v i)))
-  //   (ensures (fun h0 _ h1 -> inv h0 (v i) ))
-  // =
-  //   res.(i) <- add_zq (poly_index a i) (poly_index b i)
-  // in
-  Lib.Loops.for 0ul aDeg inv 
-  (fun i ->
-    // res.(i) <- add_zq (poly_index a i) (poly_index b i)
-    res.(i) <- u32 3328
-  )
+  let inv h (i:nat) =
+    live h a /\ live h b /\ live h res /\ modifies (loc res) h0 h in
+  let body (i: U32.t{ 0 <= U32.v i /\ U32.v i < U32.v deg }):
+    Stack unit
+    (requires (fun h -> inv h (U32.v i)))
+    (ensures (fun h0 () h1 -> inv h0 (U32.v i) /\ inv h1 (U32.v i + 1)))
+    = let ai = a.(i) in
+      let bi = b.(i) in
+      let sum = add_zq ai bi in
+      res.(i) <- sum in
+  Lib.Loops.for 0ul deg inv body;
+  pop_frame ()
