code/mlkem/Hacl.Spec.MLkem.Poly.fst
@@ -4,123 +4,20 @@ open FStar.Seq
 unfold let max = FStar.Math.Lib.max
 
 open Lib.IntTypes
+open Lib.Sequence
 
 let q: int = 3329
 let zq = x:int{ x < q && x >= 0 }
 
-let lpoly deg = (lseq zq deg)
-let zero = create 0 0
-let one = create 1 1
+let lpoly deg = lseq zq deg
 
-// let valid (s:lseq zq deg) : bool =
-//   length s = 0 || (index s (length s - 1) <> 0)
-
-
-
-val poly_index:
-    #deg:nat
-  -> p: lpoly deg
-  -> i:nat
-  -> zq
-  
-let poly_index p i =
-  if 0 <= i && i < length p then 
-  index p i
-  else 0
-
-let to_seq #deg (p:lpoly deg) : Pure (seq zq)
-  (requires True)
-  (ensures fun s ->
-    length s == deg /\
-    (forall (i:nat).{:pattern (poly_index p i) \/ (index s i)} i < length s ==> poly_index p i == index s i)
-  )
-  =
-  init deg (poly_index p)
-
-// let rec of_seq (s:lseq zq deg) : Pure poly_mod
-//   (requires True)
-//   (ensures fun p ->
-//     length p <= length s /\
-//     (forall (i:nat).{:pattern (p.[i]) \/ (index s i)} i < length s ==> p.[i] == index s i)
-//   )
-//   (decreases (length s))
-//   =
-//   if length s < deg 
-//   then init deg (fun i -> if i < length s then s.[i] else 0)
-//   else
-//     of_seq (slice s 0 (length s - 1))
-
-// let rec of_seq (s:seq zq) : Pure poly_mod
-//   (requires True)
-//   (ensures fun p ->
-//     length p <= length s /\
-//     (forall (i:nat).{:pattern (p.[i]) \/ (index s i)} i < length s ==> p.[i] == index s i)
-//   )
-//   (decreases (length s))
-//   =
-//   if valid s then s
-//   else
-//     of_seq (slice s 0 (length s - 1))
-
-[@"opaque_to_smt"]
-// let of_fun (len:nat) (f:nat -> zq) : Pure poly_mod
-let of_fun (#deg:nat) (f:nat -> zq) : Pure (lpoly deg)
-  (requires True)
-  (ensures fun p ->
-    // length p <= len /\
-    (forall (i:nat).{:pattern poly_index p i \/ (f i)} i < deg ==> poly_index p i == f i) /\
-    (forall (i:nat).{:pattern poly_index p i} (poly_index p i <> 0) ==> 0 <= i /\ i < deg)
-  )
-  =
-  init deg f
-  // of_seq (init len f)
-
-val get_lowest_n: #deg:nat -> p:lpoly deg -> n:nat -> Pure (lseq zq n)
-  (requires True)
-  (ensures fun s ->
-    length s == n /\
-    (forall (i:nat).{:pattern (poly_index p i) \/ (index s i)} i < n ==> poly_index p i == index s i)
-  )
-let get_lowest_n #deg p n =
-  if n <= deg then
-    (slice p 0 n)
-  else append p (create (n - deg) 0)
-
-val add_zq: a:zq -> b:zq -> Pure zq
-  (requires True)
-  (ensures fun r -> r == (a + b) % q)
+val add_zq: a:zq -> b:zq -> zq
 let add_zq a b = (a + b) % q
 
-val add: #aDeg:size_nat 
-  -> #bDeg:size_nat{bDeg <= aDeg} 
-  -> a:lpoly aDeg
-  -> b:lpoly bDeg
-  -> Pure (lpoly aDeg) 
-  (requires True)
-  (ensures fun p ->
-    let len = max (length a) (length b) in
-    length p <= len /\
-    (forall (i:nat).{:pattern poly_index p i} poly_index p i == (poly_index a i + poly_index b i) % q)
-  )
-let add #aDeg #bDeg a b = 
-  let len = max (length a) (length b) in
-  of_fun (fun (i:nat) -> (poly_index a i + poly_index b i) % q)
-
-// // f j + f (j + 1) + ... + f (k - 1)
-// let rec sum_element (j k: int) (f: int -> int) : Tot int (decreases (k -j)) = 
-//   if j >= k then 0
-//   else (sum_element j (k-1) f) + f (k - 1)
-
-// // a0 * bk + a1 * b(k-1) + ... + ak * b0
-// let mul_element (a b:poly_mod) (k:int) : zq = 
-//   (sum_element 0 (k+1) (fun i -> (a.[i] * b.[k - i]))) % q
-
-// let mul (a b:poly_mod) : Pure poly_mod
-//   (requires True)
-//   (ensures fun p ->
-//     let len = length a + length b in
-//     length p <= len /\
-//     (forall (i:nat).{:pattern p.[i]} i < len ==> p.[i] == mul_element a b i)
-//   ) =
-//   let len = length a + length b in
-//   of_fun len (fun (i:nat) -> mul_element a b i)
+val add:
+    #deg:size_nat
+  -> a:lpoly deg
+  -> b:lpoly deg
+  -> lpoly deg
+let add #deg a b =
+  createi deg (fun i -> add_zq (index a i) (index b i))
